Progressing on algebraic hierarchy.

theories/Fun.ec
@@ -7,256 +7,74 @@
  * the ssreflect library that is (c) Copyright Microsoft Corporation
  * and Inria. *)
 
-require import ExtEq.
-require import Option.
+(* -------------------------------------------------------------------- *)
+require import ExtEq Option.
 
-(*** Properties of functions (see ssrfun) *)
-(** Definitions *)
-(* id<:'a> is the identity function on 'a *)
+(* -------------------------------------------------------------------- *)
 op id (x:'a) = x.
 
-(* preim f p x <=> x is in the preimage of p by f *)
+(* -------------------------------------------------------------------- *)
 pred preim ['a 'b] (f : 'a -> 'b) p x = p (f x).
 
-(** Definitions for composition *)
-theory Composition.
-  op comp (g:'b -> 'c) (f:'a -> 'b): ('a -> 'c) =
-    fun x, g (f x).
+(* -------------------------------------------------------------------- *)
+op (\o) ['a 'b 'c] (g : 'b -> 'c) (f : 'a -> 'b) =
+  fun x => g (f x).
 
-  op pcomp (f:'b -> 'a option) (g:'c -> 'b option) x =
-    obind f (g x).
+op (\c) ['a 'b 'c] (f : 'b -> 'a option) (g : 'c -> 'b option) =
+  fun x => obind f (g x).
 
-  lemma eq_comp (f:'b -> 'a) f' (g:'c -> 'b) g':
-    f == f' =>
-    g == g' =>
-    comp f g == comp f' g'.
-  proof. by move=> eq_ff' eq_gg' x; rewrite /comp eq_gg' eq_ff'. qed.
-end Composition.
-export Composition.
+(* -------------------------------------------------------------------- *)
+lemma comp_eqE ['a 'b 'c] (f f' : 'b -> 'a) (g g' : 'c -> 'b):
+  f == f' => g == g' => (f \o g) == (f' \o g').
+proof. by do 2! (move/fun_ext=> ->). qed.
 
-theory Morphism.
-  (** Morphisms *)
-  (* Morphism property for unary and binary functions *)
-  pred morphism_1 (f:'a -> 'b) aF rF =
-    forall x, f (aF x) = rF (f x).
+(* -------------------------------------------------------------------- *)
+pred morphism_1 (f : 'a -> 'b) aF rF =
+  forall x, f (aF x) = rF (f x).
 
-  pred morphism_2 (f:'a -> 'b) aOp rOp =
-    forall x y, f (aOp x y) = rOp (f x) (f y).
+pred morphism_2 (f : 'a -> 'b) aOp rOp =
+  forall x y, f (aOp x y) = rOp (f x) (f y).
 
-  (* Homomorphism property for unary and binary relations *)
-  pred homomorphism_1 (f:'a -> 'b) aP rP =
-    forall x, aP x => rP (f x).
+pred homomorphism_1 (f : 'a -> 'b) aP rP =
+  forall x, aP x => rP (f x).
 
-  pred homomorphism_2 (f:'a -> 'b) aR rR =
-    forall x y, aR x y => rR (f x) (f y).
+pred homomorphism_2 (f : 'a -> 'b) aR rR =
+  forall x y, aR x y => rR (f x) (f y).
 
-  (* Stability property for unary and binary relations *)
-  pred monomorphism_1 (f:'a -> 'b) (aP: 'a -> 'c) rP =
-    forall x, rP (f x) = aP x.
+pred monomorphism_1 (f : 'a -> 'b) (aP : 'a -> 'c) rP =
+  forall x, rP (f x) = aP x.
 
-  pred monomorphism_2 (f:'a -> 'b) (aR:'a -> 'a -> 'c) rR =
-    forall x y, rR (f x) (f y) = aR x y.
-end Morphism.
-export Morphism.
+pred monomorphism_2 (f : 'a -> 'b) (aR : 'a -> 'a -> 'c) rR =
+  forall x y, rR (f x) (f y) = aR x y.
 
-theory Injections.
-  pred injective (f:'a -> 'b) =
-    forall (x y:'a), f x = f y => x = y.
+(* -------------------------------------------------------------------- *)
+ pred injective (f : 'a -> 'b) =
+   forall x y, f x = f y => x = y.
 
-  pred cancel (f:'a -> 'b) (g:'b -> 'a) =
-    forall x, g (f x) = x.
+ pred cancel (f : 'a -> 'b) (g : 'b -> 'a) =
+   forall x, g (f x) = x.
 
-  pred pcancel (f:'a -> 'b) (g:'b -> 'a option) =
-    forall x, g (f x) = Some x.
+ pred pcancel (f : 'a -> 'b) (g : 'b -> 'a option) =
+   forall x, g (f x) = Some x.
 
-  pred ocancel (g:'b -> 'a option) h =
-    forall x, oapp h x (g x) = x.
+ pred ocancel (g : 'b -> 'a option) h =
+   forall x, oapp h x (g x) = x.
 
-  lemma nosmt can_pcan (f:'a -> 'b) g: cancel f g => pcancel f (fun y, Some (g y)).
-  proof. by move=> fK x //=; rewrite fK. qed.
+(* -------------------------------------------------------------------- *)
+lemma nosmt can_pcan (f:'a -> 'b) g: cancel f g => pcancel f (Some \o g).
+proof. by move=> fK x; rewrite /(\o) fK. qed.
 
-  lemma nosmt pcan_inj (f:'a -> 'b) g: pcancel f g => injective f.
-  proof.
-    move=> fK x y h; apply (congr1 g) in h.
-    by generalize h; rewrite !fK.
-  qed.
+lemma nosmt pcan_inj (f:'a -> 'b) g: pcancel f g => injective f.
+proof. by move=> fK x y /(congr1 g); rewrite !fK. qed.
 
-  lemma nosmt can_inj (f : 'a -> 'b) g: cancel f g => injective f.
-  proof. by move=> h; apply can_pcan in h; apply pcan_inj in h. qed.
+lemma nosmt can_inj (f : 'a -> 'b) g: cancel f g => injective f.
+proof. by move/can_pcan/pcan_inj. qed.
 
-  lemma nosmt canLR (f:'a -> 'b) g x y: cancel f g => x = f y => g x = y.
-  proof. by move=> fK ->; rewrite fK. qed.
+lemma nosmt canLR (f:'a -> 'b) g x y: cancel f g => x = f y => g x = y.
+proof. by move=> fK ->; rewrite fK. qed.
 
-  lemma nosmt canRL (f:'a -> 'b) g x y: cancel f g => f x = y => x = g y.
-  proof. by move=> fK <-; rewrite fK. qed.
-end Injections.
-export Injections.
-
-theory InjectionsTheory.
-  lemma nosmt inj_id: injective (id<:'a>).
-  proof. by []. qed.
-
-  lemma nosmt inj_can_sym (f:'a -> 'b) f': cancel f f' => injective f' => cancel f' f.
-  proof. by move=> fK injf' x; apply injf'; rewrite fK. qed.
-
-  lemma nosmt inj_comp (f:'b -> 'a) (h:'c -> 'b): injective f => injective h => injective (comp f h).
-  proof. by move=> injf injh x y hy; apply injf in hy; apply injh. qed.
-
-  lemma nosmt can_comp (f:'b -> 'a) (h:'c -> 'b) f' h':
-    cancel f f' => cancel h h' => cancel (comp f h) (comp h' f').
-  proof. by move=> fK hK x; rewrite /comp /comp fK hK. qed.
-
-  lemma nosmt pcan_pcomp (f:'b -> 'a) (h:'c -> 'b) f' h':
-    pcancel f f' => pcancel h h' => pcancel (comp f h) (pcomp h' f').
-  proof. by move=> fK hK x; rewrite /comp /pcomp fK /= hK. qed.
-
-  lemma nosmt eq_inj (f g:'a -> 'b): injective f => f == g => injective g.
-  proof. by move=> injf eqfg x y; rewrite -2!eqfg; apply injf. qed.
-
-  lemma nosmt eq_can (f g:'a -> 'b) f' g': cancel f f' => f == g => f' == g' => cancel g g'.
-  proof. by move=> fK eqfg eqfg' x; rewrite -eqfg -eqfg' fK. qed.
-
-  lemma nosmt inj_can_eq (f g:'a -> 'b) f': cancel f f' => injective f' => cancel g f' => f == g.
-  proof. by move=> fK injf' gK x; apply injf'; rewrite fK gK. qed.
-end InjectionsTheory.
-export InjectionsTheory.
-
-theory Bijections.
-  pred bijective (f:'b -> 'a) = exists g,
-    cancel f g /\ cancel g f.
-
-  lemma nosmt bij_inj (f:'b -> 'a): bijective f => injective f.
-  proof. by case=> g [fK _]; apply (can_inj f g). qed.
-
-  lemma nosmt bij_can_sym (f:'b -> 'a) f': bijective f => (cancel f' f <=> cancel f f').
-  proof.
-    intros=> bijf; split=> fK; first by apply inj_can_sym; [apply fK | apply bij_inj].
-    by case bijf=> h [_ hK] x; rewrite -hK fK.
-  qed.
-
-  lemma nosmt bij_can_eq (f:'b -> 'a) f' f'': bijective f => cancel f f' => cancel f f'' => f' == f''.
-  proof.
-    move=> bijf.
-    rewrite -bij_can_sym // => fK.
-    rewrite -bij_can_sym // => fK'.
-    by apply (inj_can_eq f' f'' f)=> //; apply bij_inj.
-  qed.
-end Bijections.
-export Bijections.
-
-theory BijectionsTheory.
-  lemma nosmt eq_bij (f:'b -> 'a): bijective f => forall g, f == g => bijective g.
-  proof.
-    case=> f' [fK f'K] g eqfg; exists f'; split.
-      by apply (eq_can f _ f').
-      by apply (eq_can f' _ f).
-  qed.
-
-  lemma nosmt bij_comp (f:'b -> 'a) (h:'c -> 'b): bijective f => bijective h => bijective (comp f h).
-  proof.
-  by move=> [f' [fK f'K]] [h' [hK h'K]]; exists (comp h' f'); split; apply can_comp.
-  qed.
-
-  lemma nosmt bij_can_bij (f:'b -> 'a): bijective f => forall f', cancel f f' => bijective f'.
-  proof.
-    case=> f' [fK f'K] g gK.
-    cut eqf'g:= bij_can_eq f f' g _ _ _=> //; first by exists f'.
-    by exists f; split; [apply (eq_can f' _ f) | apply (eq_can f _ f')].
-  qed.
-end BijectionsTheory.
-export BijectionsTheory.
-
-theory Involutions.
-  pred involutive (f:'a -> 'a) = cancel f f.
-
-  lemma nosmt inv_inj (f:'a -> 'a): involutive f => injective f.
-  proof. by apply can_inj. qed.
-
-  lemma nosmt inv_bij (f:'a -> 'a): involutive f => bijective f.
-  proof. by move=> invf; exists f. qed.
-end Involutions.
-export Involutions.
-
-theory OperationProperties.
-  theory SopTisR.
-    pred left_inverse (e:'a) (inv:'a -> 'a) (o:'a -> 'a -> 'a) =
-      forall (x:'a), o (inv x) x = e.
-
-    pred right_inverse (e:'a) (inv:'a -> 'a) (o:'a -> 'a -> 'a) =
-      forall (x:'a), o x (inv x) = e.  
-
-    pred left_injective (o:'a -> 'a -> 'a) =
-      forall (x y z:'a), o x y = o z y => x = z.
-
-    pred right_injective (o:'a -> 'a -> 'a) =
-      forall (x y z:'a), o x y = o x z => y = z.
-  end SopTisR.
-  export SopTisR.
-
-  theory SopTisS.
-    pred right_id e (o:'a -> 'b -> 'a) =
-      forall x, o x e = x.
-
-    pred left_zero z (o:'a -> 'b -> 'a) =
-      forall x, o z x = z.
-
-    pred right_commutative (o:'a -> 'b -> 'a) =
-      forall x y z, o (o x y) z = o (o x z) y.
-
-    pred left_distributive (o1:'a -> 'b -> 'a) (o2:'a -> 'a -> 'a) =
-      forall x y z, o1 (o2 x y) z = o2 (o1 x z) (o1 y z).
-
-    pred right_loop inv (o:'a -> 'b -> 'a) =
-      forall y, cancel (fun x, o x y) (fun x, o x (inv y)).
-
-    pred rev_right_loop inv (o:'a -> 'b -> 'a) =
-      forall y, cancel (fun x, o x (inv y)) (fun x, o x y).
-  end SopTisS.
-  export SopTisS.
-
-  theory SopTisT.
-    pred left_id e (o:'a -> 'b -> 'b) =
-      forall x, o e x = x.
-
-    pred right_zero z (o:'a -> 'b -> 'b) =
-      forall x, o x z = z.
-
-    pred left_commutative (o:'a -> 'b -> 'b) =
-      forall x y z, o x (o y z) = o y (o x z).
-
-    pred right_distributive (o:'a -> 'b -> 'b) add =
-      forall x y z, o x (add y z) = add (o x y) (o x z).
-
-    pred left_loop inv (o:'a -> 'b -> 'b) =
-      forall x, cancel (o x) (o (inv x)).
-
-    pred rev_left_loop inv (o:'a -> 'b -> 'b) =
-      forall x, cancel (o (inv x)) (o x).
-  end SopTisT.
-  export SopTisT.
-
-  theory SopSisT.
-    pred self_inverse e (o:'a -> 'a -> 'b) =
-     forall x, o x x = e.
-
-    pred commutative (o:'a -> 'a -> 'b) =
-      forall x y, o x y = o y x.
-  end SopSisT.
-  export SopSisT.
-
-  theory SopSisS.
-    pred idempotent (o:'a -> 'a -> 'a) =
-      forall x, o x x = x.
-
-    pred associative (o:'a -> 'a -> 'a) =
-      forall x y z, o x (o y z) = o (o x y) z.
-
-    pred interchange op1 op2 =
-      forall (x:'a) y z t, op1 (op2 x y) (op2 z t) = op2 (op1 x z) (op1 y t).
-  end SopSisS.
-  export SopSisS.
-end OperationProperties.
-export OperationProperties.
+lemma nosmt canRL (f:'a -> 'b) g x y: cancel f g => f x = y => x = g y.
+proof. by move=> fK <-; rewrite fK. qed.
 
 lemma nosmt inj_eq (f : 'a -> 'b):
   injective f => forall x y, (f x = f y) <=> (x = y).
@@ -269,3 +87,172 @@ proof. by move=> can_fg; apply inj_eq; apply (can_inj f g). qed.
 lemma nosmt can2_eq (f : 'a -> 'b) g:
   cancel f g => cancel g f => forall x y, (f x = y) <=> (x = g y).
 proof. by move=> fK gK x y; rewrite -{1}gK; apply (can_eq f g). qed.
+
+(* -------------------------------------------------------------------- *)
+lemma nosmt inj_id: injective (id<:'a>).
+proof. by []. qed.
+
+lemma nosmt inj_can_sym (f:'a -> 'b) f':
+  cancel f f' => injective f' => cancel f' f.
+proof. by move=> fK injf' x; apply injf'; rewrite fK. qed.
+
+lemma nosmt inj_comp (f:'b -> 'a) (h:'c -> 'b):
+  injective f => injective h => injective (f \o h).
+proof. by move=> injf injh x y /injf /injh. qed.
+
+lemma nosmt can_comp (f:'b -> 'a) (h:'c -> 'b) f' h':
+  cancel f f' => cancel h h' => cancel (f \o h) (h' \o f').
+proof. by move=> fK hK x; rewrite /(\o) fK hK. qed.
+
+lemma nosmt pcan_pcomp (f:'b -> 'a) (h:'c -> 'b) f' h':
+  pcancel f f' => pcancel h h' => pcancel (f \o h) (h' \c f').
+proof. by move=> fK hK x; rewrite /(\o) /(\c) fK /= hK. qed.
+
+lemma nosmt eq_inj (f g:'a -> 'b):
+  injective f => f == g => injective g.
+proof. by move=> injf eqfg x y; rewrite -2!eqfg; apply injf. qed.
+
+lemma nosmt eq_can (f g:'a -> 'b) f' g':
+  cancel f f' => f == g => f' == g' => cancel g g'.
+proof. by move=> fK eqfg eqfg' x; rewrite -eqfg -eqfg' fK. qed.
+
+lemma nosmt inj_can_eq (f g:'a -> 'b) f':
+  cancel f f' => injective f' => cancel g f' => f == g.
+proof. by move=> fK injf' gK x; apply injf'; rewrite fK gK. qed.
+
+(* -------------------------------------------------------------------- *)
+pred bijective ['a 'b] (f : 'b -> 'a) = exists g, cancel f g /\ cancel g f.
+
+lemma nosmt bij_inj (f:'b -> 'a): bijective f => injective f.
+proof. by case=> g [fK _]; apply (can_inj f g). qed.
+
+lemma nosmt bij_can_sym (f:'b -> 'a) f':
+  bijective f => (cancel f' f <=> cancel f f').
+proof.
+  move=> bij_f; have /bij_inj inj_f := bij_f.
+  split=> fK; 1: by apply/inj_can_sym.
+  by case: bij_f=> h [_ hK] x; rewrite -hK fK.
+qed.
+
+lemma nosmt bij_can_eq (f:'b -> 'a) f' f'':
+  bijective f => cancel f f' => cancel f f'' => f' == f''.
+proof.
+  move=> big_j fK fK'; apply/(inj_can_eq _ _ f);
+    by rewrite 1?bij_can_sym //; apply/bij_inj.
+qed.
+
+(* -------------------------------------------------------------------- *)
+lemma nosmt eq_bij (f:'b -> 'a):
+  bijective f => forall g, f == g => bijective g.
+proof.
+  case=> f' [fK f'K] g eqfg; exists f'; split.
+  by apply (eq_can f _ f'). by apply (eq_can f' _ f).
+qed.
+
+lemma nosmt bij_comp (f:'b -> 'a) (h:'c -> 'b):
+  bijective f => bijective h => bijective (f \o h).
+proof.
+  move=> [f' [fK f'K]] [h' [hK h'K]].
+  by exists (h' \o f'); split; apply can_comp.
+qed.
+
+lemma nosmt bij_can_bij (f:'b -> 'a):
+  bijective f => forall f', cancel f f' => bijective f'.
+proof. by move=> bij_f f' can_ff'; exists f; rewrite bij_can_sym. qed.
+
+(* -------------------------------------------------------------------- *)
+pred involutive (f:'a -> 'a) = cancel f f.
+
+lemma nosmt inv_inj (f:'a -> 'a): involutive f => injective f.
+proof. by apply can_inj. qed.
+
+lemma nosmt inv_bij (f:'a -> 'a): involutive f => bijective f.
+proof. by move=> invf; exists f. qed.
+
+(* -------------------------------------------------------------------- *)
+pred left_inverse (e:'a) (inv:'a -> 'a) (o:'a -> 'a -> 'a) =
+  forall (x:'a), o (inv x) x = e.
+
+pred right_inverse (e:'a) (inv:'a -> 'a) (o:'a -> 'a -> 'a) =
+  forall (x:'a), o x (inv x) = e.  
+
+pred left_inverse_in (p : 'a -> bool) (e : 'a) inv (o : 'a -> 'a -> 'a) =
+  forall x, p x => o (inv x) x = e.
+
+pred right_inverse_in (p : 'a -> bool) (e : 'a) inv (o : 'a -> 'a -> 'a) =
+  forall x, p x => o x (inv x) = e.
+
+pred left_injective (o:'a -> 'a -> 'a) =
+  forall (x y z:'a), o y x = o z x => y = z.
+
+pred right_injective (o:'a -> 'a -> 'a) =
+  forall (x y z:'a), o x y = o x z => y = z.
+
+pred left_injective_in p (o:'a -> 'a -> 'a) =
+  forall x, p x => forall y z, o y x = o z x => y = z.
+
+pred right_injective_in p (o:'a -> 'a -> 'a) =
+  forall x, p x => forall y z, o x y = o x z => y = z.
+
+pred right_id e (o:'a -> 'b -> 'a) =
+  forall x, o x e = x.
+
+pred left_zero z (o:'a -> 'b -> 'a) =
+  forall x, o z x = z.
+
+pred right_commutative (o:'a -> 'b -> 'a) =
+  forall x y z, o (o x y) z = o (o x z) y.
+
+pred left_distributive (o1:'a -> 'b -> 'a) (o2:'a -> 'a -> 'a) =
+  forall x y z, o1 (o2 x y) z = o2 (o1 x z) (o1 y z).
+
+pred right_loop (inv : 'b -> 'b) (o:'a -> 'b -> 'a) =
+  forall y, cancel (fun x, o x y) (fun x, o x (inv y)).
+
+pred rev_right_loop inv (o:'a -> 'b -> 'a) =
+  forall y, cancel (fun x, o x (inv y)) (fun x, o x y).
+
+pred left_loop inv (o:'a -> 'b -> 'b) =
+  forall x, cancel (o x) (o (inv x)).
+
+pred rev_left_loop inv (o:'a -> 'b -> 'b) =
+  forall x, cancel (o (inv x)) (o x).
+
+pred right_loop_in p (inv : 'b -> 'b) (o:'a -> 'b -> 'a) =
+  forall y, p y => cancel (fun x, o x y) (fun x, o x (inv y)).
+
+pred rev_right_loop_in p inv (o:'a -> 'b -> 'a) =
+  forall y, p y => cancel (fun x, o x (inv y)) (fun x, o x y).
+
+pred left_loop_in p inv (o:'a -> 'b -> 'b) =
+  forall x, p x => cancel (o x) (o (inv x)).
+
+pred rev_left_loop_in p inv (o:'a -> 'b -> 'b) =
+  forall x, p x => cancel (o (inv x)) (o x).
+
+pred left_id e (o:'a -> 'b -> 'b) =
+  forall x, o e x = x.
+
+pred right_zero z (o:'a -> 'b -> 'b) =
+  forall x, o x z = z.
+
+pred left_commutative (o:'a -> 'b -> 'b) =
+  forall x y z, o x (o y z) = o y (o x z).
+
+pred right_distributive (o:'a -> 'b -> 'b) add =
+  forall x y z, o x (add y z) = add (o x y) (o x z).
+
+pred self_inverse e (o:'a -> 'a -> 'b) =
+ forall x, o x x = e.
+
+pred commutative (o:'a -> 'a -> 'b) =
+  forall x y, o x y = o y x.
+
+pred idempotent (o:'a -> 'a -> 'a) =
+  forall x, o x x = x.
+
+pred associative (o:'a -> 'a -> 'a) =
+  forall x y z, o x (o y z) = o (o x y) z.
+
+pred interchange op1 op2 =
+  forall (x:'a) y z t, op1 (op2 x y) (op2 z t) = op2 (op1 x z) (op1 y t).
