theories/core/ExtEq.ec
@@ -3,27 +3,31 @@
  * Distributed under the terms of the CeCILL-C license
  * -------------------------------------------------------------------- *)
 
-(** Extensional equality for functions *)
-(* This is separate from more advanced
-   definitions and results on functions
-   to avoid sending large amounts of stuff
-   to SMT whenever possible. *)
+(* Extensional equality for functions.
+ *
+ * This is separate from more advanced definitions and results on
+ * functions to avoid sending large amounts of stuff to SMT whenever
+ * possible.
+ *)
+
+(* -------------------------------------------------------------------- *)
 pred (==) (f g:'a -> 'b) = forall x, f x = g x.
 
-lemma nosmt frefl  (X:'a -> 'b):     X == X by [].
-lemma nosmt fsym   (X Y:'a -> 'b):   X == Y => Y == X by [].
-lemma nosmt ftrans (X Y Z:'a -> 'b): X == Y => Y == Z => X == Z by [].
+(* -------------------------------------------------------------------- *)
+lemma nosmt frefl  (f     : 'a -> 'b): f == f by [].
+lemma nosmt fsym   (f g   : 'a -> 'b): f == g => g == f by [].
+lemma nosmt ftrans (f g h : 'a -> 'b): f == g => g == h => f == h by [].
 
-axiom fun_ext (f g:'a -> 'b): f == g <=> f = g.
+(* -------------------------------------------------------------------- *)
+axiom fun_ext ['a 'b] (f g:'a -> 'b): f == g <=> f = g.
 
-(* Congruence when assumption is extensional *)
-lemma congr_ext (f g:'a -> 'b) (x y:'a):
-  f == g => x = y => f x = g y
-by rewrite fun_ext=> -> ->.
+(* -------------------------------------------------------------------- *)
+lemma econgr1 ['a 'b] (f g : 'a -> 'b) x y: f == g => x = y => f x = g y.
+proof. by move/fun_ext=> -> ->. qed.
 
-(* We need to have these two explicit, since = is not an operator *)
-lemma eqL (x:'a): (fun y, x = y) = (=) x
-by apply fun_ext.
+(* -------------------------------------------------------------------- *)
+lemma eqL (x:'a): (fun y => x = y) = (=) x.
+proof. by apply fun_ext. qed.
 
-lemma eqR (y:'a): (fun x, x = y) = (=) y
-by (apply fun_ext=> x //=; rewrite (eq_sym x)).
+lemma eqR (y:'a): (fun x => x = y) = (=) y.
+proof. by apply fun_ext=> x; rewrite (eq_sym x). qed.
